\documentclass{article}
\usepackage[utf8]{inputenc}
\documentclass{article}
\usepackage{indentfirst}
\usepackage{geometry}
\usepackage{ntheorem}
\usepackage{amsmath}
\usepackage{amssymb}

\geometry{left=3cm,right=2.5cm,top=2.5cm,bottom=2.5cm}
% \indent
\newtheorem*{proposition}{Proposition}
\newtheorem*{definition}{Definition}
\newtheorem*{corrolary}{Corrolary}
\newtheorem*{consider}{Consider}
\newtheorem*{theorem}{Theorem}
\newtheorem*{suppose}{Suppose}
\newtheorem*{notice}{Notice}
\newtheorem*{define}{Define}
\newtheorem*{denote}{Denote}
\newtheorem*{lemma}{Lemma}
\newtheorem*{claim}{Claim}
\newtheorem*{proof}{Proof}
\newtheorem*{case}{Case}
\newtheorem*{skill}{Skill}
\newtheorem*{axiom}{Axiom}
\newtheorem*{algorithm}{Algorithm}
\def\theo{\begin{theorem}}
\def\ax{\begin{axiom}}
\def\alg{\begin{algorithm}}
\def\pro{\begin{proof} }
\def\cla{\begin{claim}}
\def\sk{\begin{skill}}
\def\prop{\begin{proposition}}
\def\defi{\begin{definition}}
\def\lem{\begin{lemma}}
\def\cor{\begin{corrolary}}
\def\den{\begin{denote}}
\def\define{\begin{define}}
\def\supp{\begin{suppose}}
\def\enu{\begin{enumerate} \end{enumerate}}
\def\RR{\mathbb{R}}
\def\ZZ{\mathbb{Z}}
\def\NN{\mathbb{N}}
\def\QQ{\mathbb{Q}}
\def\CC{\mathbb{C}}
\def\FF{\mathbb{F}}
\def\KK{\mathbb{K}}
\def\calBB{\mathcal{B}}
\def\calCC{\mathcal{C}}
\def\calLL{\mathcal{L}}
\def\calPP{\mathcal{P}}
\def\implies{\Longrightarrow}
\def\bfit#1{\textit{\textbf{#1}}}
\DeclareSymbolFont{largesymbolsA}{U}{txexa}{m}{n}
\DeclareMathSymbol{\varprod}{\mathop}{largesymbolsA}{16}
\title{ECE 491}
\author{Zhihao Wang}
\date{Feb 2023}

\begin{document}

\maketitle

\subsection*{1 Proof}
$\forall \delta \in [-\Delta, \Delta]$, we can fix one of this $\delta$, then we can get this inequality, 
\[
\begin{split}
|p(x) - \tilde{p}(x)| &= |\sum \limits_{i=0}^{n-1} a_ix^i - \sum \limits_{i=0}^{n-1} (a_i + \delta_ia_i)x^i| \\ 
&=|\sum \limits_{i=0}^{n-1} a_ix^i - \sum \limits_{i=0}^{n-1} (a_i + \delta_ia_i)x^i| \\ 
&=|\sum \limits_{i=0}^{n-1} \delta_ia_ix^i| \\
&\le \sum \limits_{i=0}^{n-1}| \delta_ia_ix^i|  \\
&\le \max_i |\delta_i|  \sum \limits_{i=0}^{n-1}| a_ix^i| 
\end{split}
\]
We can get equality under some circumstance, then we know that we have,

\[
\begin{split}
\max \limits_{\delta \in [-\Delta, \Delta]^n} \frac{|p(x) - \tilde{p}(x)| / |p(x)|}{\max_i |\delta_i|} =  \frac{\max_i |\delta_i|  \sum \limits_{i=0}^{n-1}| a_ix^i|  / |p(x)|}{ \max_i |\delta_i|}  = \frac{\sum \limits_{i=0}^{n-1}| a_ix^i| }{|p(x)|}
\end{split}
\]

Which means,

$$\text{LHS} = \frac{\sum \limits_{i=0}^{n-1}| a_ix^i| }{|p(x)|} =  \frac{\sum \limits_{i=0}^{n-1}| a_ix^i| }{|\sum \limits_{i=0}^{n-1} a_ix^i |} = \text{RHS}$$

\subsection*{2 Proof}


% Now, since $\tilde{p}(x) = 0$, we know,
% $$|p(x) - \tilde{p}(x)| =|\sum \limits_{i=0}^{n-1} \delta_ia_ix^i| = |\sum \limits_{i=0}^{n-1} a_ix^i|$$



Since we know $\text{K}_{rel} \times \text{Backward ERR}_{Rel} \ge \text{Forward ERR}_{Rel} $, and $\tilde p(x) = 0$ we we have, 
$$k(p, x) \cdot d(p, \tilde p) \ge \frac{p(x) - \tilde p(x)}{p(x)} = \frac{p(x)}{p(x)} = 1$$

So, we have,
$$k(p, x) \ge \frac{1}{d(p, \tilde p)}$$

Now, we need to calculate the distance,

\[
\begin{split}
d(p, \tilde{p}) = \max \limits_{i \in {\{1, ..., n -1\}}} \frac{|a_i - \delta_ia_i - a_i|}{|a_i|} =  \max \limits_{i \in {\{1, ..., n -1\}}} \frac{|\delta_ia_i|}{|a_i|} =  \max \limits_{i \in {\{1, ..., n -1\}}} |\delta_i|
\end{split}
\]

From part1, we know the expression of $|p(x) - \tilde{p}(x)|$, which is,

$$|p(x) - \tilde{p}(x)| =|\sum \limits_{i=0}^{n-1} \delta_ia_ix^i| $$

Since $\tilde{p}(x) = 0$, we know,

$$|p(x) - \tilde{p}(x)| = |p(x)| \implies |p(x)| = |p - \tilde p(x)| =  |\sum \limits_{i=0}^{n-1} \delta_ia_ix^i| = |\sum \limits_{i=0}^{n-1} a_ix^i| $$

From the definition of $k(p, x)$, we have, 
\[
\begin{split}
k(p, x) = \max \limits_{\delta \in [-\Delta, \Delta]^n} \frac{|p(x) - \tilde{p}(x)| / |p(x)|}{\max_i |\delta_i|} = \max \limits_{\delta \in [-\Delta, \Delta]^n} \frac{1}{d(p, \tilde p)}
\end{split}
\]

Which means, $k(p, x)$ can reach the value $\frac{1}{d(p, \tilde p)}$, W.R.T some $\delta$,

So that, $$k(p, x) = \frac{\sum \limits_{i = 0}^{n-1}|a_ix^i|}{|p(x)|} = \frac{1}{d(p, \tilde p)}$$

% From part1, we know the inequality of $|p(x) - \tilde{p}(x)|$, which is,

% $$|p(x) - \tilde{p}(x)| \le \max_i |\delta_i|  \sum \limits_{i=0}^{n-1}| a_ix^i| = d(p, \tilde{p}) |p(x)|$$

% Since $\tilde{p}(x) = 0$, we know,



\end{document}
